kalloc/ASI_kalloc.v
@@ -33,14 +33,14 @@ Variable kfreeID: ident.
 
 Definition kfree_spec' := 
   DECLARE kfreeID
-      WITH n:Z, new_head:val, gv:globals, sh:share, ls: list val, xx:Z, original_freelist_pointer:val
+      WITH n:Z, new_head:val, gv:globals, sh:share, ls: list val, xx:Z, orig_head:val
       PRE [ tptr tvoid]
         PROP(
               is_pointer_or_null new_head
               ) 
         PARAMS (new_head) GLOBALS(gv)
         SEP (
-          mem_mgr K gv sh ls xx original_freelist_pointer;
+          mem_mgr K gv sh ls xx orig_head;
           if eq_dec new_head nullval then emp
           else (kalloc_token' K sh n new_head)
         )
@@ -49,32 +49,32 @@ Definition kfree_spec' :=
         RETURN () 
         SEP (
           if eq_dec new_head nullval then 
-          mem_mgr K gv sh ls xx original_freelist_pointer
+          mem_mgr K gv sh ls xx orig_head
           else 
             (
-              mem_mgr K gv sh (original_freelist_pointer::ls) xx new_head
+              mem_mgr K gv sh (orig_head::ls) xx new_head
             )).
 
 
 Definition kalloc_spec' :=
 DECLARE kallocID
-WITH n:Z, gv:globals, sh:share, ls: list val, xx:Z, original_freelist_pointer:val
+WITH n:Z, gv:globals, sh:share, ls: list val, xx:Z, orig_head:val
 PRE [ ]
     PROP(0 < n <= PGSIZE)
     PARAMS () GLOBALS(gv)
-    SEP ( mem_mgr K gv sh ls xx original_freelist_pointer
+    SEP ( mem_mgr K gv sh ls xx orig_head
     )  
 POST [ tptr tvoid ]
     PROP()
-    RETURN (original_freelist_pointer) 
+    RETURN (orig_head) 
     SEP (
-      if (eq_dec original_freelist_pointer nullval) then
-        (mem_mgr K gv sh ls xx original_freelist_pointer)
+      if (eq_dec orig_head nullval) then
+        (mem_mgr K gv sh ls xx orig_head)
       else 
         (
           EX next ls',
           (!! (next :: ls' = ls) &&
-              kalloc_token' K sh n original_freelist_pointer *
+              kalloc_token' K sh n orig_head *
               mem_mgr K gv sh ls' xx next 
           )
         )
