kalloc/Verif_kfree_loops_examples.v
@@ -18,7 +18,7 @@ Local Open Scope logic.
 
 Definition kfree_kfree_kalloc_loop_spec := 
     DECLARE _kfree_kfree_kalloc_loop
-    WITH sh : share, pa1:val, original_freelist_pointer:val, xx:Z, gv:globals, ls : list val, next:val
+    WITH sh : share, pa1:val, orig_head:val, xx:Z, gv:globals, ls : list val, next:val
     PRE [ tptr tvoid ]
         PROP(
             isptr pa1 /\ (* just assume it is pointers for simplicity *)
@@ -27,7 +27,7 @@ Definition kfree_kfree_kalloc_loop_spec :=
         PARAMS (pa1) GLOBALS(gv)
         SEP (
             kalloc_tokens Tok_APD sh (2)%nat pa1 PGSIZE t_run *
-            KAF_globals gv sh ls xx original_freelist_pointer
+            KAF_globals gv sh ls xx orig_head
         )
     POST [ tptr tvoid ]
         PROP( )
@@ -36,12 +36,12 @@ Definition kfree_kfree_kalloc_loop_spec :=
             (
                 (*data_at sh t_run pa1 (offset_val PGSIZE pa1) **)
                 kalloc_token' KAF_APD sh (sizeof t_run) (offset_val PGSIZE pa1) *
-                KAF_globals gv sh (original_freelist_pointer::ls) xx pa1
+                KAF_globals gv sh (orig_head::ls) xx pa1
                 ).
 
 Definition kfree_loop_spec := 
     DECLARE _kfree_loop
-    WITH sh : share, pa1:val, original_freelist_pointer:val, xx:Z, gv:globals, ls : list val, n:Z
+    WITH sh : share, pa1:val, orig_head:val, xx:Z, gv:globals, ls : list val, n:Z
     PRE [ tptr tvoid, tint ]
         PROP(
             isptr pa1 /\
@@ -51,13 +51,13 @@ Definition kfree_loop_spec :=
         PARAMS (pa1; Vint (Int.repr n)) GLOBALS(gv)
         SEP (
             kalloc_tokens Tok_APD sh (Z.to_nat n)%nat pa1 PGSIZE t_run *
-            KAF_globals gv sh ls xx original_freelist_pointer
+            KAF_globals gv sh ls xx orig_head
         )
     POST [ tvoid ]
         EX head, EX added_elem, (* TODO: fix top and next is the same?? *)
         PROP( 
-            added_elem = (pointers_with_original_head (Z.to_nat n) (pa1) PGSIZE original_freelist_pointer) /\
-            head = (hd nullval ((pointers_with_original_head (Z.to_nat n+1) (pa1) PGSIZE original_freelist_pointer)++ls))
+            added_elem = (pointers_with_original_head (Z.to_nat n) (pa1) PGSIZE orig_head) /\
+            head = (hd nullval ((pointers_with_original_head (Z.to_nat n+1) (pa1) PGSIZE orig_head)++ls))
             )
             RETURN () (* we return the head like in the pop function*)
             SEP 
@@ -67,7 +67,7 @@ Definition kfree_loop_spec :=
 
 Definition kfree_loop_kalloc_spec := 
     DECLARE _kfree_loop_kalloc
-    WITH sh : share, pa1:val, original_freelist_pointer:val, xx:Z, gv:globals, ls : list val, n:Z
+    WITH sh : share, pa1:val, orig_head:val, xx:Z, gv:globals, ls : list val, n:Z
     PRE [ tptr tvoid, tint ]
         PROP(
             isptr pa1 /\
@@ -77,26 +77,26 @@ Definition kfree_loop_kalloc_spec :=
         PARAMS (pa1; Vint (Int.repr n)) GLOBALS(gv)
         SEP (
             kalloc_tokens Tok_APD sh (Z.to_nat n)%nat pa1 PGSIZE t_run *
-            KAF_globals gv sh ls xx original_freelist_pointer
+            KAF_globals gv sh ls xx orig_head
         )
     POST [ tptr tvoid ]
         EX head, EX added_elem, (* TODO: fix top and next is the same?? *)
         PROP( 
             (* before alloc *)
-            added_elem = (pointers_with_original_head (Z.to_nat n) (pa1) PGSIZE original_freelist_pointer) /\
-            head = (hd nullval ((pointers_with_original_head (Z.to_nat n+1) (pa1) PGSIZE original_freelist_pointer)++ls))
+            added_elem = (pointers_with_original_head (Z.to_nat n) (pa1) PGSIZE orig_head) /\
+            head = (hd nullval ((pointers_with_original_head (Z.to_nat n+1) (pa1) PGSIZE orig_head)++ls))
             )
             RETURN (head) (* we return the head like in the pop function*)
             SEP 
             (
             let n_eq_0_case :=
-                if eq_dec original_freelist_pointer nullval then
-                emp * KAF_globals gv sh ls xx original_freelist_pointer
+                if eq_dec orig_head nullval then
+                emp * KAF_globals gv sh ls xx orig_head
             else
                 EX next, EX ls',
                     !! (next :: ls' = ls) &&
                     KAF_globals gv sh ls' xx next *
-                    kalloc_token' KAF_APD sh (sizeof t_run) original_freelist_pointer
+                    kalloc_token' KAF_APD sh (sizeof t_run) orig_head
             in
             let n_gt_0_case :=
                 KAF_globals gv sh ((tl added_elem)++ls) xx (hd nullval added_elem) *
@@ -120,8 +120,8 @@ Proof.
     (EX i:Z, EX p_tmp:val, EX curr_head:val, EX tmp_added_elem : list val,
     PROP  (
         0 <= i <= 2 /\
-        ((curr_head = original_freelist_pointer /\ i = 0) \/ (curr_head = (offset_val (-PGSIZE) (p_tmp))  /\ i <> 0)) /\
-        tmp_added_elem = (pointers_with_original_head (Z.to_nat i) (pa1) PGSIZE original_freelist_pointer) /\
+        ((curr_head = orig_head /\ i = 0) \/ (curr_head = (offset_val (-PGSIZE) (p_tmp))  /\ i <> 0)) /\
+        tmp_added_elem = (pointers_with_original_head (Z.to_nat i) (pa1) PGSIZE orig_head) /\
         p_tmp = offset_val (i * PGSIZE)%Z pa1 /\
         Int.min_signed <=
         Int.signed (Int.repr i) + Int.signed (Int.repr 1) <=
@@ -139,7 +139,7 @@ Proof.
         )
         )
     )%assert; destruct H as [H H3].
-    - entailer. Exists 0 pa1 original_freelist_pointer (pointers_with_original_head (Z.to_nat 0) pa1 PGSIZE original_freelist_pointer). (*entailer. *)
+    - entailer. Exists 0 pa1 orig_head (pointers_with_original_head (Z.to_nat 0) pa1 PGSIZE orig_head). (*entailer. *)
         rewrite <- pointers_with_head_empty. simpl; entailer!; unfold offset_val in H2; destruct pa1; auto_contradict.
     - entailer.
     - Intros. destruct (Z.to_nat (2 - i)) eqn:e.
@@ -156,7 +156,7 @@ Proof.
             unfold offset_val. destruct pa1; auto_contradict; auto.
             forward. if_tac; auto_contradict; destruct H0 as [H01 [H02 [H03 [H04 H05]]]]; rewrite H04 in H1.
                 -- unfold offset_val in H1. destruct pa1; auto_contradict.
-                -- Exists ((((i+1)%Z, (offset_val PGSIZE p_tmp):val), p_tmp:val), (curr_head::(pointers_with_original_head(Z.to_nat (i)) pa1 PGSIZE)original_freelist_pointer):list val).
+                -- Exists ((((i+1)%Z, (offset_val PGSIZE p_tmp):val), p_tmp:val), (curr_head::(pointers_with_original_head(Z.to_nat (i)) pa1 PGSIZE)orig_head):list val).
                 entailer!. 
                 ++ split; try rep_lia. split.
                     ** right. split; try rep_lia. replace (i * PGSIZE + PGSIZE + - PGSIZE) with (i * PGSIZE)%Z; try rep_lia.
@@ -176,9 +176,9 @@ Proof.
                 ++ unfold KAF_globals. 
                 assert (Z.to_nat (2 - (i + 1)) = n); try rep_lia.
                 rewrite H6. rewrite app_comm_cons. entailer!.
-    - forward_call (kalloc_spec_sub KAF_APD t_run) (gv, sh , pa1::original_freelist_pointer::ls, xx, offset_val PGSIZE pa1). (* kalloc *)
+    - forward_call (kalloc_spec_sub KAF_APD t_run) (gv, sh , pa1::orig_head::ls, xx, offset_val PGSIZE pa1). (* kalloc *)
         +
-        (*- forward_call (sh, add_offset pa1 PGSIZE, xx, (pa1::original_freelist_pointer::ls), gv). (* call kalloc *)*)
+        (*- forward_call (sh, add_offset pa1 PGSIZE, xx, (pa1::orig_head::ls), gv). (* call kalloc *)*)
         entailer. destruct H0 as [H01 [H02 [H03 [H04 H05]]]]; rewrite H04 in H1.
         unfold KAF_globals. rewrite H03.
         rewrite mem_mgr_split.
@@ -213,8 +213,8 @@ Intros. forward. (*forward. unfold abb iate in POSTCONDITION.*)
     (EX i:Z, EX p_tmp:val, EX curr_head:val, EX tmp_added_elem : list val,
     PROP  (
         0 <= i <= n /\
-        ((curr_head = original_freelist_pointer /\ i = 0) \/ (curr_head = (offset_val (-PGSIZE) (p_tmp))  /\ i <> 0)) /\
-        tmp_added_elem = (pointers_with_original_head (Z.to_nat i) (pa1) PGSIZE original_freelist_pointer) /\
+        ((curr_head = orig_head /\ i = 0) \/ (curr_head = (offset_val (-PGSIZE) (p_tmp))  /\ i <> 0)) /\
+        tmp_added_elem = (pointers_with_original_head (Z.to_nat i) (pa1) PGSIZE orig_head) /\
         p_tmp = offset_val (i * PGSIZE)%Z pa1 /\
         Int.min_signed <=
         Int.signed (Int.repr i) + Int.signed (Int.repr 1) <=
@@ -232,7 +232,7 @@ Intros. forward. (*forward. unfold abb iate in POSTCONDITION.*)
             kalloc_tokens Tok_APD sh (Z.to_nat(n-i)) p_tmp (PGSIZE) t_run
         )
     ))%assert; destruct H as [H01 [H02 H03]].
-    - entailer. Exists 0 pa1 original_freelist_pointer (pointers_with_original_head (Z.to_nat 0) pa1 PGSIZE original_freelist_pointer). (*entailer. *)
+    - entailer. Exists 0 pa1 orig_head (pointers_with_original_head (Z.to_nat 0) pa1 PGSIZE orig_head). (*entailer. *)
         rewrite <- pointers_with_head_empty. entailer. destruct (Z.to_nat n).
             + rewrite <- H0 in H01. try rep_lia.
             + rewrite app_nil_l. entailer!.
@@ -256,7 +256,7 @@ Intros. forward. (*forward. unfold abb iate in POSTCONDITION.*)
                 ++ destruct H0 as [H001 [H002 [H003 [H04 H05]]]]. rewrite H04.
                 assert ( isptr (p_tmp)). { rewrite H04. apply isptr_offset_val'. auto. }
                 rewrite H in H0; auto_contradict.
-                ++ Exists ((((i+1)%Z, (offset_val PGSIZE p_tmp):val), p_tmp:val), ((pointers_with_original_head(Z.to_nat (i+1)) pa1 PGSIZE)original_freelist_pointer):list val).
+                ++ Exists ((((i+1)%Z, (offset_val PGSIZE p_tmp):val), p_tmp:val), ((pointers_with_original_head(Z.to_nat (i+1)) pa1 PGSIZE)orig_head):list val).
                 entailer!; destruct H0 as [H001 [H002 [H003 [H04 H05]]]].
                     **simpl. do 2 split; try rep_lia. split. 
                         --- right. split. rewrite isptr_offset_val_zero; auto.
@@ -278,7 +278,7 @@ Intros. forward. (*forward. unfold abb iate in POSTCONDITION.*)
 
                     assert (Z.to_nat (n - (i + 1)) = n0); try rep_lia.
                     rewrite H0.
-                    assert (curr_head :: tmp_added_elem = pointers_with_original_head (Z.to_nat (i + 1)) pa1 PGSIZE original_freelist_pointer). {
+                    assert (curr_head :: tmp_added_elem = pointers_with_original_head (Z.to_nat (i + 1)) pa1 PGSIZE orig_head). {
                         rewrite H003.
                         destruct H002 as [[H0021 H0022] | [H0021 H0022]].
                         - rewrite H0022. simpl. rewrite H0021. auto.
@@ -310,7 +310,7 @@ Qed.
 Lemma body_kfree_loop_kalloc: semax_body KAFVprog KAFGprog_clients f_kfree_loop_kalloc kfree_loop_kalloc_spec.
 Proof.
 start_function.
-forward_call (sh, pa1:val, original_freelist_pointer:val, xx:Z, gv:globals, ls : list val, n:Z).
+forward_call (sh, pa1:val, orig_head:val, xx:Z, gv:globals, ls : list val, n:Z).
 - destruct H as [H1 [H2 H3]]; auto.
 - Intros vret. 
 forward_call (kalloc_spec_sub KAF_APD t_run) (gv, sh , snd vret ++ ls, xx,  fst vret ); (* kalloc *)
